#### Proposition â€“ Locus of a Set and Radical are Equal
For any subset $S$ of $k[x_1,\dots,x_n]$[^1] we have[^2] $$V(S) = V(\langle S\rangle) = V \left(\sqrt{\langle S\rangle}\right).$$In particular, $V(I) = V (\sqrt{I})$ for any ideal $I$.

##### *Proof.*
The containments $\supseteq$ hold since $S \sse \langle S\rangle \sse \sqrt{(S)}.$ Say $P\in V(S)$. An arbitrary element of $\langle S\rangle$ has the form $f = f_{1}g_{1}+\dots+f_{m}g_{m}$ with $f_i\in k[x_1,\dots,x_n]$ and $g_i\in S$ for all $i$. We have  $$f(P) =\sum\limits_{i} f_{i}(P)g_{i}(P) =\sum\limits_{i}f_{i}(P)\cdot0=0.$$This proves $V(S)=V(\langle S\rangle)$. Given any ideal $I$, if $P\in V(I)$ and $f$ is such that $f^n\in I$, then $f(P)^{n} = (f^{n})(P) = 0$ and hence $f(P) = 0$. This proves $V(I) = V(\sqrt{I})$.

[^1]: Notation: [[Polynomial Ring]]
[^2]: Notation: $V(S)$ denotes the [[Zero Locus]] of $S$, $\langle S\rangle$ denotes the ideal [[Generator|generated]] by $S$, $\sqrt{\langle S\rangle}$ denotes the [[Radical Ideal|radical]] of the ideal generated by $S$.